coq/core.v
@@ -1,2 +1,4 @@
+From elpi Require Export elpi.
 From Coq.Init Require Import Notations.
+
 Notation "x -> y" := (forall (_ : x), y).
