coq/elpi_exploration.v
@@ -1,0 +1,233 @@
+From Coq Require Import Prelude.
+
+Require Import core.
+From Coq.Classes Require Import CRelationClasses.
+From elpi Require Import elpi.
+
+(** Let's try and learn some Elpi. *)
+(** Elpi is a logic programming language, it is a variant of Prolog
+    which extends Prolog with functional features like lambda abstraction.
+
+    This is mostly for my own benefit, but you may gain something by following along
+    and watching me solve some simple problems using Elpi.
+
+    A good place to start with Elpi is the tutorials:
+    - #<a href="https://lpcic.github.io/coq-elpi/tutorial_elpi_lang.html">Tutorial on the Elpi programming language</a>#
+    - #<a href="https://lpcic.github.io/coq-elpi/tutorial_coq_elpi_HOAS.html">Tutorial on higher-order abstract syntax for Coq terms</a>#
+    - #<a href="https://lpcic.github.io/coq-elpi/tutorial_coq_elpi_command.html">Tutorial on Coq commands</a>#
+    - #<a href="https://lpcic.github.io/coq-elpi/tutorial_coq_elpi_tactic.html">Tutorial on Coq tactics</a>#
+    
+    In order to use Elpi to write tactics, you will need to constantly reference the Coq/Elpi API to see
+    how to accomplish certain things. The functionality available is spread out over a mix of Elpi files in the Coq-Elpi Github repository. Two important ones are
+    - #<a href="https://github.com/LPCIC/coq-elpi/blob/2ef66b2640af1e3ef2e859f7b49b40d47272e10a/builtin-doc/coq-builtin.elpi">coq-builtin.elpi</a>#
+    - #<a href="https://github.com/LPCIC/coq-elpi/blob/2ef66b2640af1e3ef2e859f7b49b40d47272e10a/elpi/coq-HOAS.elpi">coq-HOAS.elpi</a>
+
+    You may need to consult other files in the same coq-elpi/elpi directory to find definitions.
+
+    In what follows, I work through the tutorial 
+    #<a href="https://lpcic.github.io/coq-elpi/tutorial_coq_elpi_tactic.html">here</a>#
+    to the best of my ability, and work through what I find.
+
+    Let's first understand the domain modelling. A [goal] in Elpi is
+    documented 
+    #<a href="https://github.com/LPCIC/coq-elpi/blob/2ef66b2640af1e3ef2e859f7b49b40d47272e10a/builtin-doc/coq-builtin.elpi">here</a>#.
+
+    From glancing through the codebase, it seems like an idiom is that,
+    for "algebraic data types" with one constructor,
+    you give the constructor the same name as the type (a kind of punning).
+    In particular the type [goal] has a single constructor, also called [goal].
+
+    This goal wraps the following arguments:
+    - the goal context
+    - the "trigger" argument
+    - the goal formula (the type we are trying to construct an inhabitant of)
+    - the current proof, which is allowed to depend on the context hypotheses
+    - the list of arguments passed to the parent tactic
+
+    We put the "algebraic data types" in quotes because I think 
+    there is no exhaustiveness checking for constructors.
+
+    The basic architecture of an Elpi tactic is that:
+
+    - the entry point is through the distinguished predicate "solve"
+    - 
+ *)
+
+Elpi Program __ lp:{{
+    type goal goal-ctx -> term -> term -> term -> list argument -> goal.
+}}.
+
+Elpi Tactic intro1.
+
+(** Our first example will match the goal to a product type,
+    and, if it is a product we will refine it using an application.
+    The Coq "forall" binder is represented in Elpi using the
+    "prod" constant
+    #<a href="https://github.com/LPCIC/coq-elpi/blob/2ef66b2640af1e3ef2e859f7b49b40d47272e10a/builtin-doc/coq-builtin.elpi#L188">here</a>#.
+    
+    The term [forall (x: A), B] would be represented as something like
+
+    [prod `x` {{ A }} (y\ {{ B(y) }})]
+    
+    where the dependence of [B] on [x] is captured by making it a function.
+
+    It takes a (meaningless) name, the type of the parameterizing input,
+    and the return type expressed as a function of the input.
+*)
+
+Elpi Accumulate lp:{{
+    solve (goal _ _ (prod _ _ _) _ _ as G) GL :- 
+        refine (fun `X` _ _) G GL.
+}}.
+Elpi Typecheck.
+
+From Coq Require Import Logic Datatypes.
+Goal forall x y : nat, x = x.
+Proof.
+    elpi intro1.
+    elpi intro1.
+
+    Abort.
+
+Goal forall x y : nat, x = x.
+
+Elpi Tactic intro2.
+(** Same, except we introduce a fresh identifier.*)
+Elpi Accumulate lp:{{
+    solve (goal _ _ (prod _ _ _) _ _ as G) GL :- 
+        % Introduce a fresh identifier with "x" as its root.
+        coq.ltac.fresh-id "x" _ X,
+        % Get the name of the identifier.
+        coq.id->name X Y,
+        % Move the name Y into the current context.
+        refine (fun Y _ _) G GL.
+}}.
+
+Elpi Typecheck.
+Goal forall x y : nat, x = x.
+Proof.
+    elpi intro2.
+    elpi intro2.
+    Abort.
+
+Elpi Tactic intro3.
+(** Accept an argument telling us what the input should be.*)
+Elpi Accumulate lp:{{
+    solve (goal _ _ (prod _ _ _) _ (str Arg :: _) as G) GL :- 
+        coq.ltac.fresh-id Arg _ X,
+        coq.id->name X Y,
+        refine (fun Y _ _) G GL.
+}}.
+
+Elpi Typecheck.
+Goal forall x y : nat, x = x.
+Proof.
+    elpi intro3 a.
+    elpi intro3 a.
+    Abort.
+
+Elpi Tactic intro4.
+(** If the goal is a definition, unfold it to see if it exposes a forall clause. *)
+Elpi Accumulate lp:{{
+    solve (goal _ _ Goal _ _ as G) GL :- 
+        % Try to unfold Goal and get the identifier for a constant
+        Goal = global (const C),
+        % Try to unwrap the definition of the constant C, 
+        % failing if the constant is opaque
+        coq.env.const-body C (some Body),
+        % Proceed if the body is a forall type
+        Body = prod _ _ _,
+        refine (fun `a` _ _) G GL.
+}}.
+Elpi Typecheck.
+
+Definition adef := forall x :nat, x = x.
+Goal adef.
+    elpi intro4.
+    Abort.
+
+(** A nice generalization of intro4 would be to unfold the top term recursively,
+    repeatedly simplifying the term until the pattern is found.
+    It looks like the functions in coq-elpi/elpi/elpi-reduction.elpi 
+    can help with this.
+ *)
+
+Elpi Tactic rewrite1.
+
+(** Eq is a constant from the global environment whose type is an equality proof 
+    a = b. Rewrite all occurrences of b to a, going from right to left. *)
+
+Elpi Accumulate lp:{{
+    solve (goal _ _ GoalType _ [trm Eq] as G) GL :-
+        % Unpack Eq and get the global reference inside 
+        Eq = global Gref,
+        coq.env.typeof Gref EqTy, % EqTy is the declared type of Gref
+        EqTy = {{ @eq lp:Ty _ lp:Y }}, % EqTy is the type X = Y for X, Y : Ty
+        % Ty = {{ lp:{{_}} = lp:{{_}}  }},
+        % type match term -> term -> list term -> term.   % match t p [branch])
+        % This function is from coq-elpi/elpi/coq-lib.elpi
+        pi y\ copy Y y =>
+            copy GoalType (Goalfn y),
+            refine (match 
+                Eq
+                (fun _ Ty (a\ 
+                   fun _ EqTy (_\
+                     Goalfn a
+                )))
+        [{{_}}]) G GL.
+}}.
+Elpi Typecheck.
+
+
+Theorem abc : 3 = 5 - 2.
+Proof.
+    exact eq_refl.
+Qed.
+
+Goal forall A : Prop, 5 - 2 = 5 - 2 -> A.
+Proof.
+    elpi rewrite1 (abc).
+    Abort.
+
+Elpi Tactic rewrite2.
+(** Argument is the name of a hypothesis in the context,
+    whose type is of the form "forall (x : A), P = Q".
+ *)
+Elpi Accumulate lp:{{
+    solve (goal Ctx _ GoalType _ [trm Eq] as G) GL :-
+        std.mem Ctx (decl Eq _ Ty),
+        Ty = prod _ A (c\ {{ @eq lp:S lp:{{ Q0_ c}} lp:{{Q c}} }}),
+        Hole = {{ _ }}, 
+        coq.typecheck Hole A ok,
+        pi x\ (copy J x :- 
+            coq.unify-leq (Q Hole) J ok) => 
+            copy GoalType (P x),
+            if (occurs x (P x))
+            (refine (match 
+                (app [Eq, Hole])
+                (fun _ S (a\   
+                   fun _ {{ @eq lp:S lp:{{ Q0_ Hole}} lp:{{Q Hole}} }} (_\
+                     P a
+                )))
+        [{{_}}]) G GL 
+            )
+            (coq.ltac.fail _ "Couldn't unify.").
+}}.
+Elpi Typecheck.
+
+From Coq Require Import Peano.
+Goal (forall x : nat, 1 + x = x + 1) -> 
+    forall y,  2 * ((y+y) + 1) = ((y + y)+1) * 2.
+Proof.
+    intro H. 
+    intro x.
+    elpi rewrite2 (H).
+
+    (** Goal is [2 * (1 + (x + x)) = (1 + (x + x)) * 2] *)
+    Abort.
+(** Okay. I still need more practice with 
+Elpi but this is a good start. 
+We will have to continue and extend the rewrite example, and add other variations.
+*)
+(** Another good exercise would be to build a database of reflexive or symmetric relations,
+that tactics can query to dispatch certain kinds of proofs automatically.*)
